Implement Unlink
Currently doesn't recover the inode space but the machinery is there to
do so.

src/Dafny/util/std.dfy
@@ -1,4 +1,18 @@
 module Std
 {
   datatype Option<T> = Some(x:T) | None
+
+  function map_delete<K, V>(m: map<K, V>, k0: K): map<K, V>
+  {
+    map k: K | k in m && k != k0 :: m[k]
+  }
+
+  lemma map_delete_not_in<K, V>(m: map<K, V>, k0: K)
+    ensures k0 !in map_delete(m, k0)
+  {}
+
+  lemma map_delete_other<K, V>(m: map<K, V>, k0: K, k: K)
+    requires k in m && k != k0
+    ensures k in map_delete(m, k0) && map_delete(m, k0)[k] == m[k]
+  {}
 }
